isabelle/Distinct_Elems_Analysis.thy
@@ -1,0 +1,43 @@
+section \<open> TODO \<close>
+theory Distinct_Elems_Analysis
+
+imports
+  Distinct_Elems_Algo
+  Distinct_Elems_No_Fail
+  Distinct_Elems_Eager
+begin
+
+context with_threshold
+begin
+
+term "fail_or_satisfies"
+
+definition eps_F0_approx :: "real \<Rightarrow> 'a set \<Rightarrow> nat \<Rightarrow> bool" where
+  "eps_F0_approx (\<epsilon>::real) X n \<longleftrightarrow>
+    n \<in> {(1-\<epsilon>)*real (card X)..(1+\<epsilon>)*real (card X)} "
+
+lemma estimate_distinct_error_bound:
+  assumes "\<epsilon> > 0"
+  shows "
+    \<P>(n in estimate_distinct xs. n
+      |> fail_or_satisfies
+        (eps_F0_approx \<epsilon> (set xs)))
+     \<le> real (length xs) / 2 ^ threshold +
+        bar \<epsilon> thresh"
+  (is "?L \<le> ?R")
+proof -
+  
+  have "?L \<le> real (length xs) / 2 ^ threshold
+    + \<P>(n in estimate_distinct_no_fail xs.
+       n |> (eps_F0_approx \<epsilon> (set xs)))"
+    by (intro prob_estimate_distinct_fail_or_satisfies_le)
+
+  moreover have
+    "estimate_distinct_no_fail xs =
+    map_pmf get_estimate (lazy_algorithm xs)"
+    sorry
+  show ?thesis
+    sorry
+qed
+
+end
